

Yet Another Language for the Compiler Course
Introduction to language theory and compiling
Project – Part 2

Gilles GEERAERTS

Arnaud LEPONCE

2025-2026

The grammar is transformed as follows:

- Eliminate rule $\langle \text{Instruction} \rangle \rightarrow \langle \text{Call} \rangle$ as $\langle \text{Call} \rangle$ is an unproductive nonterminal.
- Separate rules for $\langle \text{ExprArith} \rangle$ according to operators precedence. The $\langle \text{Op} \rangle$ nonterminal has been removed in the process. Then transform these to remove left-recursion.
- Separate rules for $\langle \text{Cond} \rangle$ according to operators precedence (in this case there is only grouping between $|$ s and \rightarrow), then remove left-recursion. We also ensured that \rightarrow is right-associative with rule 26: in the produced parsing tree, the right hand-side of an implication will be in a $\langle \text{Cond} \rangle$ subtree.

The resulting grammar is given in Figure ???. We can show that this grammar is *LL1* by showing it is *Strong LL1*. To do this we compute for each rule $\alpha \rightarrow \beta$ the set $\text{First}^1(\beta \cdot \text{Follow}^1(\alpha))$ (see Table ???). Then for each pair of rules with the same left handside $\alpha \rightarrow \beta$ and $\alpha \rightarrow \beta'$ we check that

$$\text{First}^1(\beta \cdot \text{Follow}^1(\alpha)) \cap \text{First}^1(\beta' \cdot \text{Follow}^1(\alpha)) = \emptyset.$$

As we see, there is no conflict. Indeed, we can use these to fill up the *LL(1)* action table of Table ???.

[1]	<Program>	→ Prog [ProgName] Is <Code> End
[2]	<Code>	→ <Instruction> ; <Code>
[3]		→ ε
[4]	<Instruction>	→ <Assign>
[5]		→ <If>
[6]		→ <While>
[7]		→ <Output>
[8]		→ <Input>
[9]	<Assign>	→ [VarName] = <ExprArith>
[10]	<ExprArith>	→ <Prod> <ExprArith'>
[11]	<ExprArith'>	→ + <Prod> <ExprArith'>
[12]		→ - <Prod> <ExprArith'>
[13]		→ ε
[14]	<Prod>	→ <Atom> <Prod'>
[15]	<Prod'>	→ * <Atom> <Prod'>
[16]		→ / <Atom> <Prod'>
[17]		→ ε
[18]	<Atom>	→ [VarName]
[19]		→ [Number]
[20]		→ (<ExprArith>)
[21]		→ - <Atom>
[22]	<If>	→ If { <Cond> } Then <Code> <IfTail>
[23]	<IfTail>	→ End
[24]		→ Else <Code> End
[25]	<Cond>	→ <SimpleCond> <Cond'>
[26]	<Cond'>	→ -> <Cond>
[27]		→ ε
[28]	<SimpleCond>	→ <Cond>
[29]		→ <ExprArith> <Comp> <ExprArith>
[30]	<Comp>	→ ==
[31]		→ <=
[32]		→ <
[33]	<While>	→ While {<Cond>} Do <Code> End
[34]	<Output>	→ Print([VarName])
[35]	<Input>	→ Input([VarName])

Table 1: The YALCC modified grammar.

$\text{First}^1(\text{Prog } [\text{ProgName}] \text{ Is} \langle \text{Code} \rangle \text{ End Follow}^1(\langle \text{Program} \rangle)) = \{\text{Prog}\}$	(1)
$\text{First}^1(\langle \text{Instruction} \rangle ; \langle \text{Code} \rangle \text{ Follow}^1(\langle \text{Code} \rangle)) = \{[\text{VarName}], \text{If}, \text{While}, \text{Print}, \text{Input}\}$	(2)
$\text{First}^1(\varepsilon \text{ Follow}^1(\langle \text{Code} \rangle)) = \{\text{End}, \text{Else}\}$	(3)
$\text{First}^1(\langle \text{Assign} \rangle \text{ Follow}^1(\langle \text{Instruction} \rangle)) = \{[\text{VarName}]\}$	(4)
$\text{First}^1(\langle \text{If} \rangle \text{ Follow}^1(\langle \text{Instruction} \rangle)) = \{\text{If}\}$	(5)
$\text{First}^1(\langle \text{While} \rangle \text{ Follow}^1(\langle \text{Instruction} \rangle)) = \{\text{While}\}$	(6)
$\text{First}^1(\langle \text{Output} \rangle \text{ Follow}^1(\langle \text{Instruction} \rangle)) = \{\text{Print}\}$	(7)
$\text{First}^1(\langle \text{Input} \rangle \text{ Follow}^1(\langle \text{Instruction} \rangle)) = \{\text{Input}\}$	(8)
$\text{First}^1([\text{VarName}] = \langle \text{ExprArith} \rangle \text{ Follow}^1(\langle \text{Assign} \rangle)) = \{[\text{VarName}]\}$	(9)
$\text{First}^1(\langle \text{Prod} \rangle \langle \text{ExprArith}' \rangle \text{ Follow}^1(\langle \text{ExprArith} \rangle)) = \{[\text{VarName}], [\text{Number}], (, -)\}$	(10)
$\text{First}^1(+ \langle \text{Prod} \rangle \langle \text{ExprArith}' \rangle \text{ Follow}^1(\langle \text{ExprArith}' \rangle)) = \{+\}$	(11)
$\text{First}^1(- \langle \text{Prod} \rangle \langle \text{ExprArith}' \rangle \text{ Follow}^1(\langle \text{ExprArith}' \rangle)) = \{-\}$	(12)
$\text{First}^1(\varepsilon \text{ Follow}^1(\langle \text{ExprArith}' \rangle)) = \{;,), ==, <=, <, , ->, \}$	(13)
$\text{First}^1(\langle \text{Atom} \rangle \langle \text{Prod}' \rangle \text{ Follow}^1(\langle \text{Prod} \rangle)) = \{[\text{VarName}], [\text{Number}], (, -)\}$	(14)
$\text{First}^1(* \langle \text{Atom} \rangle \langle \text{Prod}' \rangle \text{ Follow}^1(\langle \text{Prod}' \rangle)) = \{*\}$	(15)
$\text{First}^1(/ \langle \text{Atom} \rangle \langle \text{Prod}' \rangle \text{ Follow}^1(\langle \text{Prod}' \rangle)) = \{/ \}$	(16)
$\text{First}^1(\varepsilon \text{ Follow}^1(\langle \text{Prod}' \rangle)) = \{+, -, ;,), ==, <=, <, , ->, \}$	(17)
$\text{First}^1([\text{VarName}] \text{ Follow}^1(\langle \text{Atom} \rangle)) = \{[\text{VarName}]\}$	(18)
$\text{First}^1([\text{Number}] \text{ Follow}^1(\langle \text{Atom} \rangle)) = \{[\text{Number}]\}$	(19)
$\text{First}^1((\langle \text{ExprArith} \rangle) \text{ Follow}^1(\langle \text{Atom} \rangle)) = \{(\}$	(20)
$\text{First}^1(- \langle \text{Atom} \rangle \text{ Follow}^1(\langle \text{Atom} \rangle)) = \{-\}$	(21)
$\text{First}^1(\text{If} \{ \langle \text{Cond} \rangle \} \text{Then} \langle \text{Code} \rangle \langle \text{IfTail} \rangle \text{ Follow}^1(\langle \text{If} \rangle)) = \{\text{If}\}$	(22)
$\text{First}^1(\text{End} \text{ Follow}^1(\langle \text{IfTail} \rangle)) = \{\text{End}\}$	(23)
$\text{First}^1(\text{Else} \langle \text{Code} \rangle \text{End} \text{ Follow}^1(\langle \text{IfTail} \rangle)) = \{\text{Else}\}$	(24)
$\text{First}^1(\langle \text{SimpleCond} \rangle \langle \text{Cond}' \rangle \text{ Follow}^1(\langle \text{Cond} \rangle)) = \{ , [\text{VarName}], [\text{Number}], (, -)\}$	(25)
$\text{First}^1(-> \langle \text{Cond} \rangle \text{ Follow}^1(\langle \text{Cond}' \rangle)) = \{->\}$	(26)
$\text{First}^1(\varepsilon \text{ Follow}^1(\langle \text{Cond}' \rangle)) = \{ \}, \}$	(27)
$\text{First}^1(\langle \text{Cond} \rangle \text{ Follow}^1(\langle \text{SimpleCond} \rangle)) = \{ \}$	(28)
$\text{First}^1(\langle \text{ExprArith} \rangle \langle \text{Comp} \rangle \langle \text{ExprArith} \rangle \text{ Follow}^1(\langle \text{SimpleCond} \rangle)) = \{[\text{VarName}], [\text{Number}], (, -)\}$	(29)
$\text{First}^1(== \text{ Follow}^1(\langle \text{Comp} \rangle)) = \{==\}$	(30)
$\text{First}^1(<= \text{ Follow}^1(\langle \text{Comp} \rangle)) = \{<=\}$	(31)
$\text{First}^1(< \text{ Follow}^1(\langle \text{Comp} \rangle)) = \{<\}$	(32)
$\text{First}^1(\text{While} \{ \langle \text{Cond} \rangle \} \text{Do} \langle \text{Code} \rangle \text{End} \text{ Follow}^1(\langle \text{While} \rangle)) = \{\text{While}\}$	(33)
$\text{First}^1(\text{Print}([\text{VarName}]) \text{ Follow}^1(\langle \text{Output} \rangle)) = \{\text{Print}\}$	(34)
$\text{First}^1(\text{Input}([\text{VarName}]) \text{ Follow}^1(\langle \text{Output} \rangle)) = \{\text{Input}\}$	(35)

Table 2: Sets $\text{First}^1(\beta \cdot \text{Follow}^1(\alpha))$ for all rules $\alpha \rightarrow \beta$.

	Prog	Is	End	If	Then	Else	While	Do	Print	Input	;	=	+	-	*	/	()	{	}	==	<=	<	->		[ProgName]	[VarName]	[Number]
<Program>	1																											
<Code>			3	2		3	2		2	2																	2	
<Instruction>				5			6		7	8																	4	
<Assign>																											9	
<ExprArith>														10			10										10	10
<ExprArith'>											13		11	12				13		13	13	13	13	13	13			
<Prod>														14			14										14	14
<Prod'>											17		17	17	15	16		17		17	17	17	17	17	17			
<Atom>														21			20										18	19
<If>				22																								
<IfTail>			23			24																						
<Cond>														25			25								25		25	25
<Cond'>																			27					26	27			
<SimpleCond>														29			29								28		29	29
<Comp>																					30	31	32					
<While>							33																					
<Output>									34																			
<Input>										35																		

Table 3: Action table